formal/easycrypt/SHA3_QROM.ec
@@ -1,0 +1,14 @@
+(*
+ * SHA3 instantiation of the QROM library (production link).
+ * Unruh theories import this module (via QROM.ec) so H is SHA3-256.
+ *
+ * Check:  easycrypt -I . -I lib SHA3_QROM.ec
+ *)
+
+require import AllCore.
+require import QROMCore.
+require import SHA3.
+
+(* Re-export: H is already sha3_256 in QROMCore *)
+lemma sha3_is_ro (m : bytes) : H m = sha3_256 m.
+proof. by rewrite /H. qed.
